wip ***NO_CI***

examples/crypto/EtM.AE.fst
@@ -45,16 +45,60 @@ let mac_only_cpa_ciphers (mac:Seq.seq EtM.MAC.log_entry) (cpa:Seq.seq EtM.CPA.lo
       <==>
      (exists (p:Plain.plain). Seq.mem (CPA.Entry p (fst c)) cpa)
 
-//AE log abstracts the mac and cpa logs
-let mac_and_cpa_refine_ae (ae:Seq.seq log_entry) 
-                          (mac:Seq.seq EtM.MAC.log_entry)
-                          (cpa:Seq.seq EtM.CPA.log_entry) =
-  forall (p:Plain.plain) (c:cipher).{:pattern (Seq.mem (p, c) ae)}
-     Seq.mem (p,c) ae
-     <==>
-     (Seq.mem c mac /\
-      Seq.mem (CPA.Entry p (fst c)) cpa)
+let mac_and_cpa_refine_ae_entry (ae:log_entry)
+                                (mac:EtM.MAC.log_entry)
+                                (cpa:EtM.CPA.log_entry) =
+    let p, c = ae in
+    mac == c /\
+    CPA.Entry p (fst c) == cpa
+    
+// //AE log abstracts the mac and cpa logs
+// let mac_and_cpa_refine_ae (ae:Seq.seq log_entry) 
+//                           (mac:Seq.seq EtM.MAC.log_entry)
+//                           (cpa:Seq.seq EtM.CPA.log_entry) =
+//   forall (p:Plain.plain) (c:cipher).{:pattern (Seq.mem (p, c) ae)}
+//      Seq.mem (p,c) ae
+//      <==>
+//      (Seq.mem c mac /\
+//       Seq.mem (CPA.Entry p (fst c)) cpa)
 
+//AE log abstracts the mac and cpa logs
+let rec mac_and_cpa_refine_ae (ae_entries:Seq.seq log_entry) 
+                              (mac_entries:Seq.seq EtM.MAC.log_entry)
+                              (cpa_entries:Seq.seq EtM.CPA.log_entry)
+        : Tot Type0 (decreases (Seq.length ae_entries)) =
+  Seq.length ae_entries == Seq.length mac_entries /\
+  Seq.length mac_entries == Seq.length cpa_entries /\
+  (if Seq.length ae_entries <> 0
+   then let ae_prefix, ae_last = Seq.un_snoc ae_entries in
+        let mac_prefix, mac_last = Seq.un_snoc mac_entries in
+        let cpa_prefix, cpa_last = Seq.un_snoc cpa_entries in
+        mac_and_cpa_refine_ae_entry ae_last mac_last cpa_last /\
+        mac_and_cpa_refine_ae ae_prefix mac_prefix cpa_prefix
+   else True)
+
+let un_snoc_snoc (#a:Type) (s:seq a) (x:a) : Lemma (un_snoc (snoc s x) == (s, x)) =
+  let s', x = un_snoc (snoc s x) in
+  assert (Seq.equal s s')
+
+let extend_ae_refinement (ae_entries:Seq.seq log_entry) 
+                         (mac_entries:Seq.seq EtM.MAC.log_entry)
+                         (cpa_entries:Seq.seq EtM.CPA.log_entry)
+                         (ae:log_entry)
+                         (mac:EtM.MAC.log_entry)
+                         (cpa:EtM.CPA.log_entry)
+    : Lemma (requires (mac_and_cpa_refine_ae ae_entries mac_entries cpa_entries /\
+                       mac_and_cpa_refine_ae_entry ae mac cpa))
+            (ensures (mac_and_cpa_refine_ae (snoc ae_entries ae)
+                                            (snoc mac_entries mac)
+                                            (snoc cpa_entries cpa)))
+    = un_snoc_snoc ae_entries ae;
+      un_snoc_snoc mac_entries mac;
+      un_snoc_snoc cpa_entries cpa
+
+// let extend_mac_cpa_relation (mac_entries: Seq.seq EtM.MAC.log_entry)
+//                             (cpa_entries: Seq.seq EtM.CPA.log_entry)
+                            
 let invariant (h:mem) (k:key) =
   let log = get_log h k in
   let mac_log = get_mac_log h k in
@@ -102,12 +146,15 @@ val encrypt: k:key -> m:Plain.plain -> ST cipher
 
 // #set-options "--initial_fuel 0 --max_fuel 0 --initial_ifuel 1 --max_ifuel 1 --z3rlimit 100"
 let encrypt k plain =
+  let h0 = FStar.HyperStack.ST.get () in
   let c = CPA.encrypt k.ke plain in
   let t = MAC.mac k.km c in
   write_at_end k.log (plain, (c, t));
-  let h = FStar.HyperStack.ST.get () in
-  assert (EtM.CPA.invariant (Key?.ke k) h);
-  admit();
+  let h1 = FStar.HyperStack.ST.get () in
+  assert (EtM.CPA.invariant (Key?.ke k) h1);
+  extend_ae_refinement (get_log h0 k) (get_mac_log h0 k) (get_cpa_log h0 k)
+                       (plain, (c,t)) (c,t) (CPA.Entry plain c);
+  assume (mac_only_cpa_ciphers (get_mac_log h1 k) (get_cpa_log h1 k));                       
   (c, t)
 
 val decrypt: k:key -> c:cipher -> ST (option Plain.plain)
@@ -119,6 +166,5 @@ val decrypt: k:key -> c:cipher -> ST (option Plain.plain)
      Seq.mem (Some?.v res, c) (get_log h0 k))))
 let decrypt k (c,tag) =
   if MAC.verify k.km c tag
-  then let msg = CPA.decrypt k.ke c in
-       Some msg
+  then Some (CPA.decrypt k.ke c)
   else None
